x86/Asm.v
@@ -942,14 +942,18 @@ Definition exec_instr (f: function) (i: instruction) (rs: regset) (m: mem) : out
       Next (nextinstr rs) m
   | Pallocframe sz ofs_ra ofs_link =>
       let (m1, stk) := Mem.alloc m 0 sz in
-      let sp := Vptr stk Ptrofs.zero in
-      match Mem.storev Mptr m1 (Val.offset_ptr sp ofs_link) rs#RSP with
-      | None => Stuck
-      | Some m2 =>
-          match Mem.storev Mptr m2 (Val.offset_ptr sp ofs_ra) rs#RA with
-          | None => Stuck
-          | Some m3 => Next (nextinstr (rs #RAX <- (rs#RSP) #RSP <- sp)) m3
-          end
+      match Mem.record_frame (Mem.push_stage m1) (Mem.mk_frame sz) with
+        |None => Stuck
+        |Some m2 =>
+         let sp := Vptr stk Ptrofs.zero in
+         match Mem.storev Mptr m2 (Val.offset_ptr sp ofs_link) rs#RSP with
+         | None => Stuck
+         | Some m3 =>
+           match Mem.storev Mptr m3 (Val.offset_ptr sp ofs_ra) rs#RA with
+           | None => Stuck
+           | Some m4 => Next (nextinstr (rs #RAX <- (rs#RSP) #RSP <- sp)) m4
+           end
+         end
       end
   | Pfreeframe sz ofs_ra ofs_link =>
       match Mem.loadv Mptr m (Val.offset_ptr rs#RSP ofs_ra) with
@@ -962,7 +966,11 @@ Definition exec_instr (f: function) (i: instruction) (rs: regset) (m: mem) : out
               | Vptr stk ofs =>
                   match Mem.free m stk 0 sz with
                   | None => Stuck
-                  | Some m' => Next (nextinstr (rs#RSP <- sp #RA <- ra)) m'
+                  | Some m' =>
+                    match Mem.pop_stage m' with
+                      |None => Stuck
+                      |Some m'' => Next (nextinstr (rs#RSP <- sp #RA <- ra)) m''
+                    end
                   end
               | _ => Stuck
               end
